setup for set membership as a predicate for code_pred

src/HOL/Predicate_Compile.thy
@@ -23,4 +23,84 @@ ML_file "Tools/Predicate_Compile/predicate_compile.ML"
 
 setup Predicate_Compile.setup
 
+subsection {* Set membership as a generator predicate *}
+
+text {* 
+  Introduce a new constant for membership to allow 
+  fine-grained control in code equations. 
+*}
+
+definition contains :: "'a set => 'a => bool"
+where "contains A x \<longleftrightarrow> x : A"
+
+definition contains_pred :: "'a set => 'a => unit Predicate.pred"
+where "contains_pred A x = (if x : A then Predicate.single () else bot)"
+
+lemma pred_of_setE:
+  assumes "Predicate.eval (pred_of_set A) x"
+  obtains "contains A x"
+using assms by(simp add: contains_def)
+
+lemma pred_of_setI: "contains A x ==> Predicate.eval (pred_of_set A) x"
+by(simp add: contains_def)
+
+lemma pred_of_set_eq: "pred_of_set \<equiv> \<lambda>A. Predicate.Pred (contains A)"
+by(simp add: contains_def[abs_def] pred_of_set_def o_def)
+
+lemma containsI: "x \<in> A ==> contains A x" 
+by(simp add: contains_def)
+
+lemma containsE: assumes "contains A x"
+  obtains A' x' where "A = A'" "x = x'" "x : A"
+using assms by(simp add: contains_def)
+
+lemma contains_predI: "contains A x ==> Predicate.eval (contains_pred A x) ()"
+by(simp add: contains_pred_def contains_def)
+
+lemma contains_predE: 
+  assumes "Predicate.eval (contains_pred A x) y"
+  obtains "contains A x"
+using assms by(simp add: contains_pred_def contains_def split: split_if_asm)
+
+lemma contains_pred_eq: "contains_pred \<equiv> \<lambda>A x. Predicate.Pred (\<lambda>y. contains A x)"
+by(rule eq_reflection)(auto simp add: contains_pred_def fun_eq_iff contains_def intro: pred_eqI)
+
+lemma contains_pred_notI:
+   "\<not> contains A x ==> Predicate.eval (Predicate.not_pred (contains_pred A x)) ()"
+by(simp add: contains_pred_def contains_def not_pred_eq)
+
+setup {*
+let
+  val Fun = Predicate_Compile_Aux.Fun
+  val Input = Predicate_Compile_Aux.Input
+  val Output = Predicate_Compile_Aux.Output
+  val Bool = Predicate_Compile_Aux.Bool
+  val io = Fun (Input, Fun (Output, Bool))
+  val ii = Fun (Input, Fun (Input, Bool))
+in
+  Core_Data.PredData.map (Graph.new_node 
+    (@{const_name contains}, 
+     Core_Data.PredData {
+       intros = [(NONE, @{thm containsI})], 
+       elim = SOME @{thm containsE}, 
+       preprocessed = true,
+       function_names = [(Predicate_Compile_Aux.Pred, 
+         [(io, @{const_name pred_of_set}), (ii, @{const_name contains_pred})])], 
+       predfun_data = [
+         (io, Core_Data.PredfunData {
+            elim = @{thm pred_of_setE}, intro = @{thm pred_of_setI},
+            neg_intro = NONE, definition = @{thm pred_of_set_eq}
+          }),
+         (ii, Core_Data.PredfunData {
+            elim = @{thm contains_predE}, intro = @{thm contains_predI}, 
+            neg_intro = SOME @{thm contains_pred_notI}, definition = @{thm contains_pred_eq}
+          })],
+       needs_random = []}))
+end
+*}
+
+hide_const (open) contains contains_pred
+hide_fact (open) pred_of_setE pred_of_setI pred_of_set_eq 
+  containsI containsE contains_predI contains_predE contains_pred_eq contains_pred_notI
+
 end
